src/impl/TLS13.Impl.Server.Driver.fst
@@ -44,6 +44,8 @@ module U64 = FStar.UInt64
 module U8 = FStar.UInt8
 module V = Pulse.Lib.Vec
 module W = TLS13.Wire.Spec
+module SS = TLS13.Impl.Server.Send
+module GSHbody = TLS13.Wire.Generated.ServerHello_body
 
 type server_driver = DS.server_driver
 
