src/impl/TLS13.Impl.Server.Driver.fsti
@@ -8,6 +8,11 @@ open Pulse.Lib.Array.PtsTo
 module B = TLS13.Bytes
 module Bounds = TLS13.Impl.ConnectionState.Bounds
 module CL = TLS13.ConnectionLog
+module CryptoSpec = TLS13.Crypto.Spec
+module M = TLS13.Messages
+module W = TLS13.Wire.Spec
+module SS = TLS13.Impl.Server.Send
+module GSHbody = TLS13.Wire.Generated.ServerHello_body
 module CS = TLS13.Spec.ConnectionState
 module CM = TLS13.Impl.ConnectionState.Model
 module CR = TLS13.Impl.ConnectionState.Repr
